use higher order functions instead of functional relations

theories/SetModel/ZF_CwF.v
@@ -1,7 +1,3 @@
-Set Primitive Projections.
-Set Universe Polymorphism.
-Set Definitional UIP.
-
 Require Import library.
 Require Import ZF_axioms.
 Require Import ZF_library.
@@ -63,3 +59,108 @@ Proof.
 Qed.
 
 (* Presheaf of types *)
+
+(* Remember: a type [A] at level i is a pair of two elements of [𝕍ᵢ] *)
+(* Then the relation [Γ ⊢ t : A] is defined to be [∀ ρ : {Γ}, {t}ρ ∈ fst {A}ρ ]*)
+
+Definition cwfTy (n : nat) (Γ : ZFSet) := Γ ⇒ (𝕍 n × 𝕍 n).
+
+Definition cwfTy_reindex (n : nat) (Γ A Δ σ : ZFSet) := setCompArr Δ Γ (𝕍 n × 𝕍 n) σ A.
+
+Lemma cwfTy_reindex_typing {n : nat} {Γ A Δ σ : ZFSet} (HA : A ∈ cwfTy n Γ) (Hσ : σ ∈ cwfSub Δ Γ) :
+  cwfTy_reindex n Γ A Δ σ ∈ cwfTy n Δ.
+Proof.
+  apply setCompArr_typing ; assumption. 
+Qed.
+
+Lemma cwfTy_reindex_id {n : nat} {Γ A : ZFSet} (HA : A ∈ cwfTy n Γ) : cwfTy_reindex n Γ A Γ (setIdArr Γ) ≡ A.
+Proof.
+  apply setCompId_left. assumption.
+Qed.
+  
+Lemma cwfTy_reindex_comp {n : nat} {Γ A Δ σ Θ τ : ZFSet} (HA : A ∈ cwfTy n Γ) (Hσ : σ ∈ cwfSub Δ Γ) (Hτ : τ ∈ cwfSub Θ Δ) :
+  cwfTy_reindex n Γ A Θ (cwfComp Γ Δ Θ σ τ) ≡ cwfTy_reindex n Δ (cwfTy_reindex n Γ A Δ σ) Θ τ.
+Proof.
+  unfold cwfTy_reindex. apply sym. apply setCompAssoc ; assumption.
+Qed.
+
+(* Dependent presheaf of terms *)
+
+Definition cwfInTy (n : nat) (Γ : ZFSet) (A : ZFSet) (t : ZFSet) :=
+  ∀ γ ∈ Γ, setAppArr Γ (𝕍 n) t γ ∈ setFstPair (𝕍 n) (𝕍 n) (setAppArr Γ (𝕍 n × 𝕍 n) A γ).
+
+Definition cwfTm (n : nat) (Γ : ZFSet) (A : ZFSet) := { t ϵ Γ ⇒ (𝕍 n) ∣ cwfInTy n Γ A t }.
+
+Definition cwfTm_reindex (n : nat) (Γ t Δ σ : ZFSet) := setCompArr Δ Γ (𝕍 n) σ t.
+
+Lemma cwfTm_reindex_typing {n : nat} {Γ A t Δ σ : ZFSet} (HA : A ∈ cwfTy n Γ) (Ht : t ∈ cwfTm n Γ A) (Hσ : σ ∈ cwfSub Δ Γ) :
+  cwfTm_reindex n Γ t Δ σ ∈ cwfTm n Δ (cwfTy_reindex n Γ A Δ σ).
+Proof.
+  apply ZFincomp in Ht. destruct Ht as [ Ht1 Ht2 ]. unfold cwfInTy in Ht2.
+  apply ZFincomp. split.
+  - apply setCompArr_typing ; assumption. 
+  - unfold cwfInTy. intros δ Hδ.
+    set (γ := setAppArr Δ Γ σ δ). assert (γ ∈ Γ) as Hγ.
+    { apply setAppArr_typing ; assumption. }
+    specialize (Ht2 γ Hγ). unfold cwfTy_reindex.
+    refine (transpS (fun x => setAppArr Δ (𝕍 n) (cwfTm_reindex n Γ t Δ σ) δ ∈ setFstPair (𝕍 n) (𝕍 n) x)
+                    (sym (setCompArr_app Hσ HA Hδ)) _).
+    refine (transpS (fun x => x ∈ setFstPair (𝕍 n) (𝕍 n) (setAppArr Γ (𝕍 n × 𝕍 n) A (setAppArr Δ Γ σ δ)))
+                    (sym (setCompArr_app Hσ Ht1 Hδ)) _).
+    exact Ht2.
+Qed.
+
+Lemma cwfTm_reindex_id {n : nat} {Γ A t : ZFSet} (Ht : t ∈ cwfTm n Γ A) : cwfTm_reindex n Γ t Γ (setIdArr Γ) ≡ t.
+Proof.
+  apply setCompId_left.
+  apply ZFincomp in Ht. destruct Ht as [ Ht _ ]. exact Ht.
+Qed.
+
+Lemma cwfTm_reindex_comp {n : nat} {Γ A t Δ σ Θ τ : ZFSet} (Ht : t ∈ cwfTm n Γ A) (Hσ : σ ∈ cwfSub Δ Γ) (Hτ : τ ∈ cwfSub Θ Δ) :
+  cwfTm_reindex n Γ t Θ (cwfComp Γ Δ Θ σ τ) ≡ cwfTm_reindex n Δ (cwfTm_reindex n Γ t Δ σ) Θ τ.
+Proof.
+  unfold cwfTm_reindex. apply sym. apply setCompAssoc ; try assumption.
+  apply ZFincomp in Ht. destruct Ht as [ Ht _ ]. exact Ht.
+Qed.
+
+(* Context extension *)
+
+Definition cwfTy_to_depSet (n : nat) (Γ A : ZFSet) : ZFSet -> ZFSet :=
+  fun γ => setFstPair (𝕍 n) (𝕍 n) (setAppArr Γ (𝕍 n × 𝕍 n) A γ).
+
+Definition ctxExt (n : nat) (Γ A : ZFSet) :=
+  setSigma n Γ (cwfTy_to_depSet n Γ A).
+
+(* First projection for context extensions *)
+
+Definition ctxWk_HO (n : nat) (Γ A : ZFSet) : ZFSet -> ZFSet :=
+  fun γa => setFstSigma n Γ (cwfTy_to_depSet n Γ A) γa.
+
+Definition ctxWk (n : nat) (Γ A : ZFSet) :=
+  relToGraph (ctxExt n Γ A) Γ (HO_rel (ctxWk_HO n Γ A)).
+
+Lemma cwfTy_to_depSet_typing {n : nat} {Γ A γ : ZFSet} (HA : A ∈ cwfTy n Γ) (Hγ : γ ∈ Γ) :
+  cwfTy_to_depSet n Γ A γ ∈ 𝕍 n.
+Proof.
+  unfold cwfTy_to_depSet. apply setFstPair_typing.
+  apply setAppArr_typing ; assumption.
+Qed.
+
+Lemma ctxWk_HO_typing {n : nat} {Γ A γa : ZFSet} (HA : A ∈ cwfTy n Γ) (Hγa : γa ∈ ctxExt n Γ A) :
+  ctxWk_HO n Γ A γa ∈ Γ.
+Proof.
+  unfold ctxWk_HO. apply setFstSigma_typing. 
+  - intros γ Hγ. now apply cwfTy_to_depSet_typing.
+  - assumption.
+Qed.
+
+Lemma ctxWk_typing (n : nat) (Γ A : ZFSet) (HA : A ∈ cwfTy n Γ) : ctxWk n Γ A ∈ cwfSub (ctxExt n Γ A) Γ.
+Proof.
+  apply relToGraph_typing. apply HO_rel_typing.
+  intros γa Hγa. now apply ctxWk_HO_typing.
+Qed.
+
+(* Second projection for context extensions *)
+
+Definition ctxWk_var0_typing (n : nat) (Γ A : ZFSet) : ctxWk_var0 n Γ A ∈ cwfTm n (ctxExt n Γ A) (cwfTy_reindex A).
+  
