theories/SetModel/library.v
@@ -1,6 +1,3 @@
-Set Primitive Projections.
-Set Universe Polymorphism.
-
 (* Our model construction is supposed to take place in ZF set theory, which is a set of axioms that
    can be put on top of first order logic (FOL). However, we certainly do not want to do a deep
    embedding of FOL in the logic of Rocq!
@@ -8,25 +5,30 @@ Set Universe Polymorphism.
    of dependent types and universes) and then postulate the skolemised axioms of ZF in HOL. This
    file does the shallow embedding of HOL into Rocq.
 
-   - We use [SProp] as our type of truth values (we postulate classical logic, so it might as well
-     be [bool]).
+   - We use [SProp] as our type of truth values (note that we postulate classical logic, so
+     [SProp] becomes isomorphic to [bool]).
    - Dependent function types are not allowed, only universal quantifiers are allowed
      (i.e., we can write [forall] only when writing an inhabitant of [SProp]).
-   - We allow prenex polymorphism over [Type], but we do not use universes otherwise.
+   - We allow prenex polymorphism over [Set], but we do not use universes otherwise.
    - Inductive types are used to simulate the logical connectives [∧] [∨] [⊤] [⊥] [∃] [=].
    - Large elimination is disallowed thanks to them living in [SProp].
  *)
 
 (* Conjunction of truth values *)
-Record andS (A : SProp) (B : SProp) : SProp :=
-  mkAndS {
-      fstS : A ;
-      sndS : B ;
-    }.
+Inductive andS (A : SProp) (B : SProp) : SProp :=
+| mkAndS : A -> B -> andS A B.
 Arguments mkAndS {_} {_}.
-Arguments fstS {_} {_}.
-Arguments sndS {_} {_}.
 Notation "A ∧ B" := (andS A B) (at level 80, right associativity).
+
+Lemma fstS {A B} : A ∧ B -> A.
+Proof.
+  intros [HA HB]. exact HA.
+Qed.
+
+Lemma sndS {A B} : A ∧ B -> B.
+Proof.
+  intros [HA HB]. exact HB.
+Qed.
 
 (* Disjunction of truth values *)
 Inductive orS (A B : SProp) : SProp :=
@@ -44,43 +46,34 @@ Notation "¬ A" := (notS A) (at level 75, right associativity).
 Definition bi_impl : SProp -> SProp -> SProp := fun A B => (A -> B) ∧ (B -> A).
 Notation "A ↔ B" := (bi_impl A B) (at level 95, no associativity).
 
-Inductive eqS (A : Type) (a : A) : A -> SProp :=
+Inductive eqS (A : Set) (a : A) : A -> SProp :=
 | eqS_refl : eqS A a a.
 Arguments eqS {_}.
 Arguments eqS_refl {_}.
 Notation "x ≡ y" := (eqS x y) (at level 70, no associativity).
 
-Definition transpS {A : Type} (P : A -> SProp) {a b : A} : a ≡ b -> P a -> P b.
+Definition transpS {A : Set} (P : A -> SProp) {a b : A} : a ≡ b -> P a -> P b.
 Proof.
   intros e p. exact (eqS_sind A a (fun b _ => P b) p b e).
 Qed.
 
-Lemma sym {A : Type} {a b : A} : a ≡ b -> b ≡ a.
+Lemma sym {A : Set} {a b : A} : a ≡ b -> b ≡ a.
 Proof.
   intro e. exact (eqS_sind A a (fun b _ => b ≡ a) (eqS_refl a) b e).
 Qed.
 
-Lemma trans {A : Type} {a b c : A} : a ≡ b -> b ≡ c -> a ≡ c.
+Lemma trans {A : Set} {a b c : A} : a ≡ b -> b ≡ c -> a ≡ c.
 Proof.
   intros e1 e2. apply (transpS (fun c => a ≡ c) e2). exact e1.
 Qed.
 
-(* Record Sigma (A : Type) (B : A -> SProp) : Type := *)
-(*   mkSigma { *)
-(*       fst : A ; *)
-(*       snd : B fst ; *)
-(*     }. *)
-(* Arguments mkSigma {_} {_}. *)
-(* Arguments fst {_} {_}. *)
-(* Arguments snd {_} {_}. *)
-
-Inductive exS (A : Type) (B : A -> SProp) : SProp :=
+Inductive exS (A : Set) (B : A -> SProp) : SProp :=
 | exS_intro : forall x : A, B x -> exS A B.
 
-Definition uniqueS {A : Type} (P : A -> SProp) (x : A) :=
+Definition uniqueS {A : Set} (P : A -> SProp) (x : A) :=
   P x ∧ forall (x':A), P x' -> x ≡ x'.
 
-Definition exU (A : Type) (B : A -> SProp) : SProp := exS A (uniqueS B).
+Definition exU (A : Set) (B : A -> SProp) : SProp := exS A (uniqueS B).
 
 (* Classical logic *)
 Axiom LEM : forall (P : SProp), P ∨ (¬ P).
